prepare future use of uint32 as clause indices
* this cannot be used yes, since clauses can be tautolgies

Weidenbach_Book/Array_UInt.thy
@@ -219,4 +219,60 @@ lemma append_el_aa_u'_code[code]:
   unfolding append_el_aa_u'_def nth_u_code_def heap_array_set'_u_def
   by auto
 
+definition (in -)length_uint32_nat where
+  [simp]: \<open>length_uint32_nat C = length C\<close>
+
+definition (in -)length_u_code where
+  \<open>length_u_code C = do { n \<leftarrow> Array.len C; return (uint32_of_nat n)}\<close>
+
+lemma (in -)length_u_hnr[sepref_fr_rules]:
+  \<open>(length_u_code, RETURN o length_uint32_nat) \<in> [\<lambda>C. length C \<le> uint32_max]\<^sub>a (array_assn R)\<^sup>k \<rightarrow> uint32_nat_assn\<close>
+  supply length_rule[sep_heap_rules]
+  by sepref_to_hoare
+    (sep_auto simp: length_u_code_def array_assn_def hr_comp_def is_array_def
+      uint32_nat_rel_def list_rel_imp_same_length br_def nat_of_uint32_uint32_of_nat_id)
+
+definition length_raa_u :: \<open>'a::heap arrayO_raa \<Rightarrow> nat \<Rightarrow> uint32 Heap\<close> where
+  \<open>length_raa_u xs i = do {
+     x \<leftarrow> arl_get xs i;
+    length_u_code x}\<close>
+
+lemma length_raa_u_alt_def: \<open>length_raa_u xs i = do {
+    n \<leftarrow> length_raa xs i;
+    return (uint32_of_nat n)}\<close>
+  unfolding length_raa_u_def length_raa_def length_u_code_def
+  by auto
+lemma length_raa_rule[sep_heap_rules]:
+  \<open>b < length xs \<Longrightarrow> <arlO_assn (array_assn R) xs a> length_raa_u a b
+   <\<lambda>r. arlO_assn (array_assn R) xs a * \<up> (r = uint32_of_nat (length_rll xs b))>\<^sub>t\<close>
+  unfolding length_raa_u_alt_def length_u_code_def
+  by sep_auto
+
+definition length_rll_n_uint32 where
+  [simp]: \<open>length_rll_n_uint32 = length_rll\<close>
+
+lemma length_raa_u_hnr[sepref_fr_rules]:
+  shows \<open>(uncurry length_raa_u, uncurry (RETURN \<circ>\<circ> length_rll_n_uint32)) \<in>
+     [\<lambda>(xs, i). i < length xs \<and> length (xs ! i) \<le> uint32_max]\<^sub>a 
+       (arlO_assn (array_assn R))\<^sup>k *\<^sub>a nat_assn\<^sup>k \<rightarrow> uint32_nat_assn\<close>
+  by sepref_to_hoare  (sep_auto simp: uint32_nat_rel_def br_def length_rll_def
+      nat_of_uint32_uint32_of_nat_id)+
+
+definition nth_rll_nu where
+  \<open>nth_rll_nu = nth_rll\<close>
+
+definition nth_raa_u' where
+  \<open>nth_raa_u' xs x L =  nth_raa xs x (nat_of_uint32 L)\<close>
+
+lemma nth_raa_u'_uint_hnr[sepref_fr_rules]:
+  assumes p: \<open>is_pure R\<close>
+  shows
+    \<open>(uncurry2 nth_raa_u', uncurry2 (RETURN \<circ>\<circ>\<circ> nth_rll)) \<in>
+       [\<lambda>((l,i),j). i < length l \<and> j < length_rll l i]\<^sub>a
+       (arlO_assn (array_assn R))\<^sup>k *\<^sub>a nat_assn\<^sup>k *\<^sub>a uint32_nat_assn\<^sup>k \<rightarrow> R\<close>
+  unfolding nth_raa_u_def
+  supply nth_aa_hnr[to_hnr, sep_heap_rules]
+  using assms
+  by sepref_to_hoare (sep_auto simp: uint32_nat_rel_def br_def nth_raa_u'_def)
+
 end
